\chapter{Assignment-Numerical Techniques Solutions}
\begin{enumerate}
	\item $\left. \right. $
	\begin{answer}
		Taylor's series for $y(x)$ is given by
		\begin{align*}
		y(x)&=1+x y_{0}^{\prime}+\frac{x^{2}}{2} y_{0}^{\prime \prime}+\frac{x^{3}}{6} y_{0}^{\prime \prime \prime}+\frac{x^{4}}{24} y_{0}^{i v} \ldots \ldots \ldots\\
		y^{\prime \prime}(x)&=x y^{\prime}(x)+y(x) \Rightarrow y^{\prime \prime}(0)=x y^{\prime}(0)+y(0)=1\\
		y^{\prime \prime \prime}(x)&=x y^{\prime \prime}(x)+2 y^{\prime}(x) \Rightarrow y^{\prime \prime \prime}(0)=x y^{\prime \prime}(x)+2 y^{\prime}(0)=0\\
		y^{i v}(x)&=x y^{\prime \prime \prime}+3 y^{\prime \prime} \Rightarrow y^{i v}(0)=x y^{\prime \prime \prime}(0)+3 y^{\prime \prime}(0)=3\\
		y(x)&=1+\frac{x^{2}}{2}+\frac{x^{4}}{24}(3) \ldots \ldots \ldots\\
		\Rightarrow y(0.1)&=1.0050 \Rightarrow y(0.05)=0.5025
		\end{align*}
		So the correct answer is \textbf{Option (d)}		
	\end{answer}
	\item $\left. \right. $
	\begin{answer}
		$h=0.5$; The value of $x$ and $y$ are tabulated below:
		\begin{align*}
		\begin{tabular}{|l|l|}
		\hline$x$ & $y$ \\
		\hline $0.0$ & $1.0000$ \\
		\hline $0.5$ & $0.6667$ \\
		\hline $1.0$ & $0.5000$ \\
		\hline
		\end{tabular}\\
		\text{Simpson's }&1 / 3\text{ rule}\\
		I=\int_{x_{0}}^{x_{n}} y d x&=\frac{h}{3}\left[y_{0}+4\left(y_{1}+y_{3}+\ldots .+y_{n-1}\right)+2\left(y_{2}+y_{4}+\ldots .+y_{n-2}\right)+y_{n}\right]\\
		\Rightarrow I&=\frac{0.5}{3}[1.0000+4(0.6667)+0.5]=0.6945
		\end{align*}
			So the correct answer is \textbf{Option (a)}
	\end{answer}
		\item $\left. \right. $
	\begin{answer}$\left. \right. $\\
		\begin{minipage}{0.45\textwidth}
		\begin{align*}
		I&=\frac{2}{3}\left[y_{0}+4\left(y_{1}+y_{3}\right)+2 y_{2}+y_{4}\right]\\
		&=\frac{2}{3}\left[\frac{1}{5}+4\left(\frac{1}{9}+\frac{1}{31}\right)+2 \times \frac{1}{21}+\frac{1}{69}\right]\\
		&=\frac{2}{3}\left[\frac{1}{5}+0.5734+0.09523+0.0145\right]\\
		&=\frac{2}{3}[0.2+0.5734+0.09523+0.0145]\\
		&=\frac{2}{3} \times 0.8831=0.5887
		\end{align*}
	\end{minipage}
	\begin{minipage}{0.45\textwidth}
		\begin{align*}
		\begin{tabular}{c|c}
		$x$ & $y=\frac{1}{x^{2}+5}$ \\
		\hline 0 & $\frac{1}{5}$ \\
		2 & $\frac{1}{9}$ \\
		4 & $\frac{1}{21}$ \\
		6 & $\frac{1}{31}$ \\
		8 & $\frac{1}{69}$
		\end{tabular}
		\end{align*}
	\end{minipage}
	\\So the correct answer is \textbf{Option (a)}
	\end{answer}
	\item $\left. \right. $
	\begin{answer}
		\begin{align*}
		 y(0.01)&=1+0.1(-1)=0.99\\
		y(0.02)&=0.99+0.01(-0.99)=0.9801
		\end{align*}
		So the correct answer is \textbf{Option (c)}
	\end{answer}
	\item  $\left. \right. $
\begin{answer}
	\begin{align*}
	y(0.01)&=1+0.1(-1)=0.99\\
	y(0.02)&=0.99+0.01(-0.99)=0.9801\\
	y(0.03)&=0.9801+0.01(-0.9801)=0.9703\\
	y(0.04)&=0.9703+0.01(-0.9703)=0.9606\\
	\text{The exact solution is }y&=e^{-x}\text{ and from this the value at }x=0.04\text{ is } 0.9606
	\end{align*}
		So the correct answer is \textbf{Option (d)}
\end{answer}
	\item  $\left. \right. $
	\begin{answer}
		\begin{align*}
	\text{	First, let }t_{0}&=0, y_{0}=1,\text{ and }h=1.\text{ Thus, we have}\\
	K_{0}&=f(0,1)=1, \quad K_{1}=f(0.5,1.5)=0.25, \quad K_{2}=\mathrm{f}(0.5,1.125)=0.4375 \\
	K_{3}&=\mathrm{f}(1,1.4375)=-0.4375 \\
	&\left(K_{0}+2 K_{1}+2 K_{2}+K_{3}\right) / 6=0.3229\\
	&\text{Therefore, approximation is }y_{1}=y_{0}+h 0.3229=1.322.
		\end{align*}
			So the correct answer is \textbf{Option (c)}
	\end{answer}
		\item  $\left. \right. $
	\begin{answer}
		For this data, we have the Forward difference table\\
		\begin{tabular}{|c|c|c|c|c|c|c|}
		\hline$x_{i}$ & $y_{i}$ & $\Delta y_{i}$ & $\Delta^{2} y_{3}$ & $\Delta^{3} y_{i}$ & $\Delta^{4} y_{i}$ & $\Delta^{5} y_{i}$ \\
		\hline 0 & $1.121$ & $0.002$ & $0.0005$ & $-0.0015$ & $0.002$ & $-.0025$ \\
		\hline $0.001$ & $1.123$ & $0.0025$ & $-0.0010$ & $0.0005$ & $-0.0005$ & \\
		\hline $0.002$ & $1.1255$ & $0.0015$ & $-0.0005$ & $0.0$ & & \\
		\hline $0.003$ & $1.127$ & $0.001$ & $-0.0005$ & & & \\
		\hline $0.004$ & $1.128$ & $0.0005$ & & & & \\
		\hline $0.005$ & $1.1285$ & & & & & \\
		\hline
		\end{tabular}
		\begin{align*}
	\text{	Thus, for }x&=x_{0}+h u,\text{ where }x_{0}=0, h=0.001\text{ and }u \frac{x-x_{0}}{h}\text{ we get}\\
		P_{5}(x)=& 1.121+u \times 0.002+\frac{u(u-1)}{2}(0.0005)+\frac{u(u-1)(u-2)}{3 !} \times(-0.0015) \\
		&+\frac{u(u-1)(u-2)(u-3)}{4 !}(0.002)+\frac{u(u-1)(u-2)(u-3)(u-4)}{5 !} \times(-0.0025) .
		\intertext{Thus}
		P_{5}(0.0045)&=P_{5}(0+0.001+4.5)\\
		&=1.121+0.002 \times 4.5+\frac{0.0005}{2}+4.5 \times 3.5-\frac{0.0015}{6} \times 4.5 \times 3.5 \times 2.5\\
		&+\frac{0.002}{24} \times 4.5 \times 3.5 \times 2.5 \times 1.5-\frac{0.0025}{120} \times 4.5 \times 3.5 \times 2.5 \times 1.5 \times 0.5\\
		&=1.12840045
		\end{align*}
			So the correct answer is \textbf{Option (b)}
	\end{answer}
		\item  $\left. \right. $
	\begin{answer}
		Taylor's series for $y(x)$ is given by
		\begin{align*}
		y(x)&=1+x y_{0}^{\prime}+\frac{x^{2}}{2} y_{0}^{\prime \prime}+\frac{x^{3}}{6} y_{0}^{\prime \prime \prime}+\frac{x^{4}}{24} y_{0}^{i v} \ldots \ldots \ldots\\
		y^{\prime \prime}(x)&=x y^{\prime}(x)+y(x) \Rightarrow y^{\prime \prime}(0)=x y^{\prime}(0)+y(0)=1\\
		y^{\prime \prime \prime}(x)&=x y^{\prime \prime}(x)+2 y^{\prime}(x) \Rightarrow y^{\prime \prime \prime}(0)=x y^{\prime \prime}(x)+2 y^{\prime}(0)=0\\
		y^{i v}(x)&=x y^{\prime \prime \prime}+3 y^{\prime \prime} \Rightarrow y^{i v}(0)=x y^{\prime \prime \prime}(0)+3 y^{\prime \prime}(0)=3\\
		y(x)&=1+\frac{x^{2}}{2}+\frac{x^{4}}{24}(3) \ldots \ldots \ldots\\
		\Rightarrow y(0.1)&=1.0050
		\end{align*}
			So the correct answer is \textbf{Option (a)}
	\end{answer}
	\item  $\left. \right. $
	\begin{answer}
		\begin{align*}
		\text{Taking origin at }0.65, h&=0.01\text{ and }x=0.6538\\
		\therefore p&=\frac{0 \cdot 6538-0 \cdot 65}{0 \cdot 01}=38\\
		\text{The difference table is}&
		\end{align*}
\begin{align*}
\renewcommand*{\arraystretch}{1.5}
\begin{tabular}{|p{1cm}| p{.5cm}|p{1.5cm}|p{1.2cm} |p{1.2cm}|p{1.2cm}|p{1.2cm}|p{1.2cm}|p{1.2cm}|}
\hline
x&p&$10^7\ y$&$10^7\ \Delta y$&$10^7\ \Delta^2 y$&$10^7\ \Delta^3 y$&$10^7\ \Delta^4 y$&$10^7\ \Delta^5 y$&$10^7\ \Delta^6 y$\\
\hline
& & &76349& & & & &\\
\hline 
0.63&-2&6270463& &-955& & & &\\
\hline
& & &75394& &$-4$& & &  \\
\hline
0.64&-1&6345857& &-959& &1& & \\
\hline
& & &74435& &-3& &1& \\
\hline
0.65&0&6420292& &-962& &2& &-4 \\
\hline
 & & &73473& &-1& &-3&  \\
 \hline
 0.66&1&6493765& &-963& &-1& &  \\
 \hline
  & & &72510& &-2& & & \\
  \hline
  0.67&2&6566275& &-965& & & &  \\
  \hline
   & & &71545& & & & & \\
   \hline
    0.68&3&6637820& & & & & &  \\
    \hline
\end{tabular}
\end{align*}	
		\begin{align*}
	\intertext{	Using Gauss's forward interpolation formula}
		\frac{p(p-1)}{2 !} \Delta^{2} y&+\frac{(p+1) p(p-1)}{3 !} \Delta^{3} y-1+\cdot \\
		10^{7} y_{0} 38=6420292+(0 \cdot 38)(73473)&+\frac{(0 \cdot 38)(0 \cdot 38-1)}{2}(-962)+\cdot \cdot=6448325 \\
		\therefore y_{0} 38&=0 \cdot 6448325
		\end{align*}
			So the correct answer is \textbf{Option (a)}
	\end{answer}
\end{enumerate}
\section{Jacobian}
\begin{enumerate}
		\item  $\left. \right. $
	\begin{answer}
		\begin{align*}
		f=y^{x}, \frac{\partial f}{\partial y}&=x y^{x-1}, \frac{\partial^{2} f}{\partial x \partial y}=\frac{\partial}{\partial x}\left(y^{x-1} x\right)=y^{x-1}+x y^{x-1} \ln y\\
		\left.\frac{\partial^{2} f}{\partial x \partial y}\right|_{x=2, y=1}&=1
		\end{align*}
		So the correct answer is \textbf{Option (c)}	
	\end{answer}
		\item  $\left. \right. $
	\begin{answer}
		\begin{align*}
		\frac{\partial z}{\partial x}&=y \ln (x y)+\frac{x y}{x y} y \Rightarrow y(\ln x y+1) \Rightarrow x \frac{\partial z}{\partial x}=x y(\ln (x y+1)\\
		\frac{\partial z}{\partial y}&=x \ln (x y)+\frac{x y}{x y} x \Rightarrow x(\ln x y+1) \Rightarrow y \frac{\partial z}{\partial y}=x y(\ln (x y+1)\\
		x \frac{\partial z}{\partial x}-y \frac{\partial z}{\partial y}&=0
		\end{align*}
		So the correct answer is \textbf{Option (c)}
	\end{answer}
		\item  $\left. \right. $
	\begin{answer}
		\begin{align}
		f(x, y)&=\sum_{K=1}^{10}\left(x^{2}-y^{2}\right)^{K} \Rightarrow \frac{\partial f}{\partial x}(x, y)=\sum_{K=1}^{10} K\left(x^{2}-y^{2}\right)^{K-1}(2 x)\\
		\text{and }\frac{\partial f}{\partial y}(x, y)&=\sum_{K=1}^{10} K\left(x^{2}-y^{2}\right)^{K-1}(-2 y)\\
		\Rightarrow y \frac{\partial f}{\partial x}(x, y)&+x \frac{\partial f}{\partial y}(x, y)=0\notag
		\end{align}
			So the correct answer is \textbf{Option (d)}
	\end{answer}
		\item  $\left. \right. $
	\begin{answer}
		\begin{align*}
		\int_{z=0}^{1} \int_{y=0}^{z} \int_{x=0}^{y} x y^{2} z^{3} d x d y d z=\int_{z=0}^{1} \int_{y=0}^{z} \frac{y^{2}}{2} y^{2} z^{3} d y d z=\int_{z=0}^{1} \frac{z^{8}}{10} d z=\frac{1}{90}
		\end{align*}
		So the correct answer is \textbf{Option (a)}
	\end{answer}
		\item  $\left. \right. $
	\begin{answer}
		\begin{align*}
		\frac{\partial x}{\partial r}&=\cos \theta, \frac{\partial y}{\partial r}=\sin \theta, \frac{\partial x}{\partial \theta}=-r \sin \theta, \frac{\partial y}{\partial \theta}=r \cos \theta\text{ and}\\
		\frac{\partial z}{\partial r}&=0, \frac{\partial z}{\partial \theta}=0, \frac{\partial z}{\partial z}=1\\
		J&=\left|\begin{array}{lll}\frac{\partial x}{\partial r} & \frac{\partial x}{\partial \theta} & \frac{\partial x}{\partial z} \\ \frac{\partial y}{\partial r} & \frac{\partial y}{\partial \theta} & \frac{\partial y}{\partial z} \\ \frac{\partial z}{\partial r} & \frac{\partial z}{\partial \theta} & \frac{\partial z}{\partial \theta}\end{array}\right|=\left|\begin{array}{ccc}\cos \theta & -r \sin \theta & 0 \\ \sin \theta & \cos \theta & 0 \\ 0 & 0 & 1\end{array}\right|=r
		\end{align*}
		So the correct answer is \textbf{Option (a)}
	\end{answer}
		\item  $\left. \right. $
	\begin{answer}
		\begin{align*}
		J\left(\frac{\partial(x, y)}{\partial(u, v)}\right)&=\left(\begin{array}{ll}\frac{\partial x}{\partial u} & \frac{\partial x}{\partial v} \\ \frac{\partial y}{\partial u} & \frac{\partial y}{\partial v}\end{array}\right)=\left|\begin{array}{cc}1-v & -u \\ v & u\end{array}\right|=(u-u v)-(-u v)=u
		\end{align*}
			So the correct answer is \textbf{Option (a)}
	\end{answer}
		\item  $\left. \right. $
	\begin{answer}
		\begin{align*}
		\frac{\partial(u, v)}{\partial(r, \theta)}&=\frac{\partial(u, v)}{\partial(x, y)} \times \frac{\partial(x, y)}{\partial(r, \theta)}\\
		\frac{\partial(u, v)}{\partial(x, y)}&=\left|\begin{array}{ll}\frac{\partial u}{\partial x} & \frac{\partial u}{\partial v} \\ \frac{\partial v}{\partial x} & \frac{\partial v}{\partial y}\end{array}\right|=\left|\begin{array}{cc}2 x & -4 y \\ 4 x & -2 y\end{array}\right|=-4 x y+16 x y=12 x y \quad\text{ put }x=r \cos \theta, y=r \sin \theta\\
		J&=\frac{\partial(x, y)}{\partial(r, \theta)}=\left|\begin{array}{ll}\frac{\partial x}{\partial r} & \frac{\partial x}{\partial \theta} \\ \frac{\partial y}{\partial r} & \frac{\partial y}{\partial \theta}\end{array}\right| \Rightarrow\left|\begin{array}{cc}\cos \theta & -r \sin \theta \\ \sin \theta & r \cos \theta\end{array}\right|=r\\
		\frac{\partial(u, v)}{\partial(r, \theta)}&=\frac{\partial(u, v)}{\partial(x, y)} \times \frac{\partial(x, y)}{\partial(r, \theta)}=12 x y \cdot r=6 r^{3} \sin 2 \theta
		\end{align*}
		So the correct answer is \textbf{Option (c)}
	\end{answer}
	
	
	

	
	
	
	
	
	
	
\end{enumerate}